Updates

intermediate2/Zeta.Intermediate.Verifier.fst
@@ -293,7 +293,7 @@ let lemma_verifyepoch_preserves_ismap
                     vs_.valid ==> is_map vs_.st))
   = ()
 
-#push-options "--z3rlimit_factor 4 --query_stats"
+#push-options "--fuel 0 --ifuel 0 --query_stats"
 
 let lemma_verifiable_implies_slot_is_merkle_points_to_appfn
   (#vcfg:_)
@@ -313,23 +313,304 @@ let lemma_verifiable_implies_slot_is_merkle_points_to_appfn
     assert(contains_only_app_keys_comp st ss);
     assert(st_ == puts_store st ss ws);
 
+    let merkle_implies_non_ref (s:_)
+      : Lemma (requires (inuse_slot st s /\ is_merkle_key (stored_base_key st s)))
+              (ensures (not (S.mem s ss)))
+      = let k = stored_base_key st s in
+        if S.mem s ss then (
+          let i = S.index_mem s ss in
+          assert(contains_app_key st (S.index ss i));
+          ()
+        )
+    in
+
     let aux (s1 s2 d:_)
       : Lemma (ensures  (slot_points_to_is_merkle_points_to_local st_ s1 s2 d))
       = eliminate
         forall (s1 s2: slot_id _) (d:_). slot_points_to_is_merkle_points_to_local st s1 s2 d
         with s1 s2 d;
         puts_preserves st ss ws s1;
-        //assert(inuse_slot st s1 = inuse_slot st_ s1);
+        puts_preserves st ss ws s2;
         if points_to_dir st_ s1 d s2 then (
-          assert(inuse_slot st_ s1);
-          //assert(inuse_slot st s1);
           let k1 = stored_base_key st_ s1 in
-          admit()
+          assert(is_merkle_key k1);
+          merkle_implies_non_ref s1;
+          puts_preserves_non_ref st ss ws s1
         )
     in
     forall_intro_3 aux
 
 #pop-options
+
+let lemma_addm_identical_except2 #vcfg
+  (vs':vtls_t vcfg{vs'.valid})
+  (e: logS_entry _ {GV.AddM? e})
+  (s1:_):
+  Lemma (requires (let GV.AddM _ s s' = e in
+                  s1 <> s /\ s1 <> s' /\
+                  (GV.verify_step e vs').valid))
+        (ensures (let st' = vs'.st in
+                  let vs = GV.verify_step e vs' in
+                  let st = vs.st in
+                  empty_slot st' s1 = empty_slot st s1 /\            // empty-ness unchanged
+                  (inuse_slot st' s1 ==>
+                   stored_key st' s1 = stored_key st s1 /\
+                   stored_value st' s1 = stored_value st s1 /\
+                   add_method_of st' s1 = add_method_of st s1))) =
+  match e with
+  | GV.AddM r s s' ->
+    let amp = AMP s r s' vs' in
+    let vs = GV.verify_step e vs' in
+    let gk,gv = r in
+    let k = to_base_key gk in
+
+    (* precond is satisfied since verify_step succeeds *)
+    assert(addm_precond amp);
+
+    let st' = addm_store_pre amp in
+    let st = vs.st in
+    let d = addm_dir amp in
+    let mv' = addm_anc_val_pre amp in
+
+    if Merkle.points_to_some mv' d then (
+      if Merkle.points_to mv' d k then (
+        assert(identical_except2 st' st s s');
+        assert(get_slot st' s1 = get_slot st s1);
+        ()
+      )
+      else (
+        assert(addm_anc_points_to_desc amp);
+        if points_to_some_slot st' s' d then  (
+          assert(addm_has_desc_slot amp);
+          let sd = addm_desc_slot amp in
+          assert(identical_except3 st' st s s' sd);
+          if sd = s1 then (
+            ()
+          )
+          else
+            assert(get_slot st' s1 = get_slot st s1)
+        )
+        else (
+          assert(identical_except2 st' st s s');
+          assert(get_slot st' s1 = get_slot st s1);
+          ()
+        )
+      )
+    )
+    else (
+      assert(identical_except2 st' st s s');
+      assert(get_slot st' s1 = get_slot st s1);
+      ()
+    )
+
+#push-options "--fuel 0 --ifuel 1 --query_stats"
+
+let lemma_verifiable_implies_slot_is_merkle_points_to_addm
+  (#vcfg:_)
+  (vs:vtls_t vcfg)
+  (e: logS_entry _ {GV.AddM? e}):
+  Lemma (requires (vs.valid /\ slot_points_to_is_merkle_points_to vs.st /\
+                   (GV.verify_step e vs).valid))
+        (ensures (let vs_ = GV.verify_step e vs in
+                  slot_points_to_is_merkle_points_to vs_.st))
+  = let vs_ = GV.verify_step e vs in
+    let st = vs.st in
+    let st1 = vs_.st in
+    let GV.AddM r s s' = e in
+    let a = AMP s r s' vs in
+
+    assert(vs_ == addm r s s' vs);
+    let aux (s1 s2: slot_id _) (dx: bin_tree_dir):
+      Lemma (slot_points_to_is_merkle_points_to_local st1 s1 s2 dx) =
+      assert(slot_points_to_is_merkle_points_to_local st s1 s2 dx);
+
+      if not (points_to_dir st1 s1 dx s2) then ()
+      else if s1 = s then (
+         assert(points_to_dir st s' (addm_dir a) s2);
+         assert(slot_points_to_is_merkle_points_to_local st (addm_anc_slot a) s2 (addm_dir a));
+         assert(s2 <> s);
+         assert(s2 <> s');
+         lemma_addm_identical_except2 vs e s2
+      )
+      else if s1 = s' then (
+        if s2 = s then (
+          let mv1' = to_merkle_value (stored_value st1 s') in
+          let d = addm_dir a in
+          assert(addm_anc_val_postcond a mv1');
+
+          if d = dx then ()
+          else (
+            // let mv' = to_merkle_value (stored_value st s') in
+            // assert(desc_hash_dir mv1' dx = desc_hash_dir mv' dx);
+            assert(addm_anc_slot_points_postcond a st1);
+            assert(points_to_info st1 s' dx = points_to_info st s' dx);
+            assert(points_to_dir st1 s' dx s2);
+            assert(points_to_dir st s' dx s2);
+            ()
+          )
+        )
+        else (
+          assert(s2 <> s);
+          if s2 = s' then (
+            assert(slot_points_to_is_merkle_points_to_local st s' s' dx);
+            ()
+          )
+          else (
+            assert(get_slot st s2 = get_slot st1 s2);
+            assert(addm_anc_slot_points_postcond a st1);
+            assert(dx = other_dir (addm_dir a));
+            assert(s1 = addm_anc_slot a);
+            assert(points_to_info st1 s' dx = points_to_info st s' dx);
+            assert(points_to_dir st s' dx s2);
+            assert(stored_key st s' = stored_key st1 s');
+            ()
+          )
+        )
+      )
+      else
+        lemma_addm_identical_except2 vs e s1
+    in
+    forall_intro_3 aux
+
+#pop-options
+
+let lemma_verifiable_implies_slot_is_merkle_points_to_evictm
+  (#vcfg:_)
+  (vs:vtls_t vcfg)
+  (e: logS_entry _{GV.EvictM? e})
+  : Lemma (requires (vs.valid /\ slot_points_to_is_merkle_points_to vs.st /\
+                   (GV.verify_step e vs).valid))
+        (ensures (let vs1 = GV.verify_step e vs in
+                  slot_points_to_is_merkle_points_to vs1.st)) =
+  let vs1 = GV.verify_step e vs in
+  let st1 = vs1.st in
+  let st = vs.st in
+  match e with
+  | GV.EvictM s s' ->
+    assert(empty_slot st1 s);
+    assert(identical_except2 st st1 s s');
+    let k = stored_base_key st s in
+    let k' = stored_base_key st s' in
+    assert(is_proper_desc k k');
+    let d = desc_dir k k' in
+
+    let aux (s1 s2: slot_id _) (dx: bin_tree_dir):
+      Lemma (slot_points_to_is_merkle_points_to_local st1 s1 s2 dx) =
+
+      if not (points_to_dir st1 s1 dx s2) then ()
+      else (
+        assert(s1 <> s);
+
+        if s1 = s' then (
+          assert(dx = other_dir d);
+          assert(points_to_info st s' dx = points_to_info st1 s' dx);
+          assert(slot_points_to_is_merkle_points_to_local st s1 s2 dx);
+          ()
+        )
+        else (
+          assert(get_slot st s1 = get_slot st1 s1);
+          assert(points_to_dir st s1 dx s2);
+          assert(slot_points_to_is_merkle_points_to_local st s1 s2 dx);
+          ()
+        )
+      )
+    in
+    forall_intro_3 aux;
+    ()
+
+let lemma_verifiable_implies_slot_is_merkle_points_to_addb (#vcfg:_)
+                                                      (vs:vtls_t vcfg)
+                                                      (e: logS_entry _{GV.AddB? e}):
+  Lemma (requires (vs.valid /\ slot_points_to_is_merkle_points_to vs.st /\
+                   (GV.verify_step e vs).valid))
+        (ensures (let vs1 = GV.verify_step e vs in
+        slot_points_to_is_merkle_points_to vs1.st)) =
+  let vs1 = GV.verify_step e vs in
+  let st1 = vs1.st in
+  let st = vs.st in
+
+  match e with
+  | GV.AddB (k,v) s  _ _  ->
+    let aux (s1 s2: slot_id _) (dx: bin_tree_dir):
+      Lemma (slot_points_to_is_merkle_points_to_local st1 s1 s2 dx) =
+      if not (points_to_dir st1 s1 dx s2) then ()
+      else (
+        (* s points to nothing after addb *)
+        assert(s1 <> s);
+        assert(get_slot st s1 = get_slot st1 s1);
+        assert(slot_points_to_is_merkle_points_to_local st s1 s2 dx);
+        assert(points_to_dir st s1 dx s2);
+        ()
+      )
+    in
+    forall_intro_3 aux;
+    ()
+
+let lemma_verifiable_implies_slot_is_merkle_points_to_evictb (#vcfg:_)
+                                                      (vs:vtls_t vcfg)
+                                                      (e: logS_entry _{GV.EvictB? e}):
+  Lemma (requires (vs.valid /\ slot_points_to_is_merkle_points_to vs.st /\
+                   (GV.verify_step e vs).valid))
+        (ensures (slot_points_to_is_merkle_points_to (GV.verify_step e vs).st)) =
+  let vs1 = GV.verify_step e vs in
+  let st1 = vs1.st in
+  let st = vs.st in
+
+  match e with
+  | GV.EvictB s  _  ->
+    let aux (s1 s2: slot_id _) (dx: bin_tree_dir):
+      Lemma (slot_points_to_is_merkle_points_to_local st1 s1 s2 dx) =
+
+      if not (points_to_dir st1 s1 dx s2) then ()
+      else (
+        assert(s <> s1);
+        assert(get_slot st s1 = get_slot st1 s1);
+        assert(slot_points_to_is_merkle_points_to_local st s1 s2 dx);
+        assert(points_to_dir st s1 dx s2);
+        ()
+      )
+    in
+    forall_intro_3 aux
+
+let lemma_verifiable_implies_slot_is_merkle_points_to_evictbm (#vcfg:_)
+                                                      (vs:vtls_t vcfg)
+                                                      (e: logS_entry _{GV.EvictBM? e}):
+  Lemma (requires (vs.valid /\ slot_points_to_is_merkle_points_to vs.st /\
+                   (GV.verify_step e vs).valid))
+        (ensures (slot_points_to_is_merkle_points_to (GV.verify_step e vs).st)) =
+  let vs1 = GV.verify_step e vs in
+  let st1 = vs1.st in
+  let st = vs.st in
+
+  match e with
+  | GV.EvictBM s s'  _  ->
+    assert(identical_except2 st1 st s s');
+    let k = stored_base_key st s in
+    let k' = stored_base_key st s' in
+    assert(is_proper_desc k k');
+    let d = desc_dir k k' in
+
+    let aux (s1 s2: slot_id _) (dx: bin_tree_dir):
+      Lemma (slot_points_to_is_merkle_points_to_local st1 s1 s2 dx) =
+
+      if not (points_to_dir st1 s1 dx s2) then ()
+      else (
+        assert(s <> s1);
+        if s1 = s' then (
+          assert(dx = other_dir d);
+          assert(points_to_info st s' dx = points_to_info st1 s' dx);
+          assert(slot_points_to_is_merkle_points_to_local st s1 s2 dx);
+          ()
+        )
+        else (
+          assert(get_slot st s1 = get_slot st1 s1);
+          assert(slot_points_to_is_merkle_points_to_local st s1 s2 dx);
+          assert(points_to_dir st s1 dx s2);
+          ()
+        )
+      )
+    in
+    forall_intro_3 aux
 
 let lemma_verifiable_implies_slot_is_merkle_points_to (#vcfg:_)
                                                       (vs:vtls_t vcfg)
@@ -338,4 +619,12 @@ let lemma_verifiable_implies_slot_is_merkle_points_to (#vcfg:_)
                    (GV.verify_step e vs).valid))
         (ensures (let vs_ = GV.verify_step e vs in
                   slot_points_to_is_merkle_points_to vs_.st))
-  = admit()
+  = let open Zeta.GenericVerifier in
+    match e with
+    | RunApp _ _ _ -> lemma_verifiable_implies_slot_is_merkle_points_to_appfn vs e
+    | AddM _ _ _ -> lemma_verifiable_implies_slot_is_merkle_points_to_addm vs e
+    | AddB _ _ _ _ -> lemma_verifiable_implies_slot_is_merkle_points_to_addb vs e
+    | EvictM _ _ -> lemma_verifiable_implies_slot_is_merkle_points_to_evictm vs e
+    | EvictB _ _ -> lemma_verifiable_implies_slot_is_merkle_points_to_evictb vs e
+    | EvictBM _ _ _ -> lemma_verifiable_implies_slot_is_merkle_points_to_evictbm vs e
+    | _ -> ()
